src/program_proof/simplepb/pb_getstate_proof.v
@@ -1,0 +1,263 @@
+From Perennial.program_proof Require Import grove_prelude.
+From Goose.github_com.mit_pdos.gokv.simplepb Require Export pb.
+From Perennial.program_proof.grove_shared Require Import urpc_proof urpc_spec.
+From Perennial.program_proof.simplepb Require Export pb_ghost.
+From Perennial.program_proof.simplepb Require Import pb_marshal_proof.
+From Perennial.program_proof Require Import marshal_stateless_proof.
+From Perennial.program_proof.simplepb Require Import pb_definitions.
+
+Section pb_getstate_proof.
+Context `{!heapGS Σ, !stagedG Σ}.
+Context {pb_record:PBRecord}.
+
+Notation OpType := (pb_OpType pb_record).
+Notation has_op_encoding := (pb_has_op_encoding pb_record).
+Notation has_snap_encoding := (pb_has_snap_encoding pb_record).
+Notation has_op_encoding_injective := (pb_has_op_encoding_injective pb_record).
+Notation compute_reply := (pb_compute_reply pb_record).
+Notation pbG := (pbG (pb_record:=pb_record)).
+
+Context `{!waitgroupG Σ}.
+Context `{!pbG Σ}.
+
+(* XXX: GetState doesn't actually *need* to do any epoch comparison.
+   It could simply return the state it has and the epoch for which it is the state.
+   The issue is that an old epoch would then be able to seal future epochs,
+   which might hurt liveness.
+ *)
+(* FIXME: rename to GetStateAndSeal *)
+Lemma wp_Clerk__GetState γ γsrv ck args_ptr (epoch_lb:u64) (epoch:u64) :
+  {{{
+        "#Hck" ∷ is_Clerk ck γ γsrv ∗
+        "#Hghost_epoch_lb" ∷ is_epoch_lb γsrv epoch_lb ∗
+        "Hargs" ∷ GetStateArgs.own args_ptr (GetStateArgs.mkC epoch)
+  }}}
+    Clerk__GetState #ck #args_ptr
+  {{{
+        (reply:loc) (err:u64), RET #reply;
+        if (decide (err = U64 0)) then
+            ∃ epochacc σ enc,
+            ⌜int.nat epoch_lb ≤ int.nat epochacc⌝ ∗
+            ⌜int.nat epochacc ≤ int.nat epoch⌝ ∗
+            is_accepted_ro γsrv epochacc σ ∗
+            is_proposal_facts γ epochacc σ ∗
+            is_proposal_lb γ epochacc σ ∗
+            GetStateReply.own reply (GetStateReply.mkC 0 (length σ) enc) ∗
+            ⌜has_snap_encoding enc (fst <$> σ)⌝ ∗
+            ⌜length σ = int.nat (U64 (length σ))⌝
+          else
+            GetStateReply.own reply (GetStateReply.mkC err 0 [])
+  }}}.
+Proof.
+  iIntros (Φ) "Hpre HΦ".
+  iNamed "Hpre".
+  wp_call.
+  wp_apply (wp_ref_of_zero).
+  { done. }
+  iIntros (rep) "Hrep".
+  wp_pures.
+  iNamed "Hck".
+  wp_apply (GetStateArgs.wp_Encode with "[$Hargs]").
+  iIntros (enc_args enc_args_sl) "(%Henc_args & Henc_args_sl & Hargs)".
+  wp_loadField.
+  iDestruct (is_slice_to_small with "Henc_args_sl") as "Henc_args_sl".
+  wp_apply (wp_frame_wand with "HΦ").
+  wp_apply (wp_Client__Call2 with "Hcl_rpc [] Henc_args_sl Hrep").
+  {
+    iDestruct "Hsrv" as "[_ [_ [$ _]]]".
+  }
+  { (* Successful RPC *)
+    iModIntro.
+    iNext.
+    unfold GetState_spec.
+    iExists _, _.
+    iSplitR; first done.
+    simpl.
+    unfold GetState_core_spec.
+    iFrame "Hghost_epoch_lb".
+    iSplit.
+    { (* No error from RPC, state was returned *)
+      iIntros (?????) "???".
+      iIntros (??? Henc_reply) "Hargs_sl".
+      iIntros (?) "Hrep Hrep_sl".
+      wp_pures.
+      wp_load.
+      wp_apply (GetStateReply.wp_Decode with "[$Hrep_sl]").
+      { done. }
+      iIntros (reply_ptr) "Hreply".
+      iIntros "HΦ".
+      iApply ("HΦ" $! _ 0).
+      iExists _, _, _.
+      iFrame "Hreply".
+      iSplitR; first done.
+      iSplitR; first done.
+      eauto with iFrame.
+    }
+    { (* GetState was rejected by the server (e.g. stale epoch number) *)
+      iIntros (err) "%Herr_nz".
+      iIntros.
+      wp_pures.
+      wp_load.
+      wp_apply (GetStateReply.wp_Decode with "[-] []").
+      { eauto. }
+      iModIntro.
+      iIntros (reply_ptr) "Hreply".
+
+      iIntros "HΦ".
+      iApply ("HΦ" $! _ err).
+      destruct (decide _).
+      {
+        exfalso. done.
+      }
+      {
+        done.
+      }
+    }
+  }
+  { (* RPC error *)
+    iIntros.
+    wp_pures.
+    wp_if_destruct.
+    {
+      wp_apply (wp_allocStruct).
+      { repeat econstructor. apply zero_val_ty'. done. }
+      iIntros (reply_ptr) "Hreply".
+      iDestruct (struct_fields_split with "Hreply") as "HH".
+      iNamed "HH".
+      iIntros "HΦ".
+      iApply ("HΦ" $! _ 3).
+      iExists _. simpl. iFrame.
+      replace (zero_val (slice.T byteT)) with (slice_val Slice.nil) by done.
+      iFrame.
+      iApply is_slice_small_nil.
+      done.
+    }
+    { exfalso. done. }
+  }
+Qed.
+
+Lemma wp_Server__GetState γ γsrv s args_ptr args epoch_lb Φ :
+  is_Server s γ γsrv -∗
+  GetStateArgs.own args_ptr args -∗
+  GetState_core_spec γ γsrv args.(GetStateArgs.epoch) epoch_lb (λ reply,
+                                                          ∀ (reply_ptr:loc),
+                                                          GetStateReply.own reply_ptr reply -∗
+                                                          Φ #reply_ptr) -∗
+  WP pb.Server__GetState #s #args_ptr {{ Φ }}
+  .
+Proof.
+  iIntros "His_srv Hargs HΦ".
+  wp_call.
+  iNamed "His_srv".
+  wp_loadField.
+  wp_apply (acquire_spec with "HmuInv").
+  iIntros "[Hlocked Hown]".
+  iNamed "Hown".
+  wp_pures.
+  iNamed "Hargs".
+  wp_loadField.
+
+  (* FIXME: separate lemma; no-op spec for isEpochStale *)
+  wp_call.
+  wp_loadField.
+  wp_if_destruct.
+  { (* *)
+    wp_loadField.
+    wp_apply (release_spec with "[-HΦ]").
+    {
+      iFrame "HmuInv Hlocked".
+      iNext.
+      iExists  _, _, _, _, _, _, _.
+      iFrame "∗#%".
+    }
+    unfold GetState_core_spec.
+    iDestruct "HΦ" as "[_ HΦ]".
+    iRight in "HΦ".
+    wp_pures.
+    wp_apply (wp_allocStruct).
+    { Transparent slice.T. repeat econstructor.
+      Opaque slice.T. }
+    iIntros (reply_ptr) "Hreply".
+    iDestruct (struct_fields_split with "Hreply") as "HH".
+    iNamed "HH".
+    iApply "HΦ"; last first.
+    {
+      iExists _. iFrame.
+      replace (slice.nil) with (slice_val Slice.nil) by done.
+      iFrame.
+      simpl.
+      iApply is_slice_small_nil.
+      done.
+    }
+    simpl.
+    done.
+  }
+  wp_storeField.
+  wp_loadField.
+
+  iAssert (_) with "HisSm" as "HisSm2".
+  iNamed "HisSm2".
+  wp_loadField.
+  iDestruct "HΦ" as "[#Hepoch_lb HΦ]".
+  wp_apply ("HgetStateSpec" with "[$Hstate]").
+  {
+    iIntros "Hghost".
+    iDestruct "Hghost" as (?) "[%Heq Hghost]".
+    iDestruct (ghost_helper1 with "Hs_prop_lb Hghost") as %Hσeq.
+    {
+      apply (f_equal length) in Heq.
+      rewrite fmap_length in Heq.
+      rewrite fmap_length in Heq.
+      done.
+    }
+    rewrite Hσeq.
+    iDestruct (ghost_epoch_lb_ineq with "Hepoch_lb Hghost") as "#Hepoch_ineq".
+    iDestruct (ghost_seal with "Hghost") as "Hghost".
+    iDestruct (ghost_get_accepted_ro with "Hghost") as "#Hacc_ro".
+    replace (σ) with (σg).
+    iSplitL "Hghost".
+    {
+      iExists _.
+      iFrame.
+      iPureIntro. done.
+    }
+    iModIntro.
+
+    iCombine "Hacc_ro Hepoch_ineq" as "HH".
+    iExact "HH".
+  }
+  iIntros (??) "(Hsnap_sl & %Hsnap_enc & [Hstate HQ])".
+  iDestruct "HQ" as "[#Hacc_ro %Hineq]".
+  wp_pures.
+  wp_loadField.
+  wp_pures.
+  wp_loadField.
+
+  iLeft in "HΦ".
+  iDestruct ("HΦ" with "[% //] [%] Hacc_ro Hs_prop_facts Hs_prop_lb [%//] [%]") as "HΦ".
+  { word. }
+  { word. }
+
+  wp_apply (release_spec with "[-Hsnap_sl HΦ]").
+  {
+    iFrame "HmuInv Hlocked".
+    iNext.
+    iExists  _, _, _, _, _, _, _.
+    iFrame "∗ HisSm #%".
+  }
+  wp_apply (wp_allocStruct).
+  { Transparent slice.T. repeat econstructor.
+    Opaque slice.T. }
+  iIntros (reply_ptr) "Hreply".
+  iDestruct (struct_fields_split with "Hreply") as "HH".
+  iNamed "HH".
+  iApply "HΦ".
+  iExists _.
+  iFrame.
+  simpl.
+  rewrite Hσ_nextIndex.
+  replace (U64 (int.nat nextIndex)) with (nextIndex) by word.
+  iFrame.
+Qed.
+
+End pb_getstate_proof.
